

Sample Data: A Best-fit Curve  
 $(x_1, y_1), (x_2, y_2) \dots (x_n, y_n)$

Assume a linear model,  $\hat{y}_i = mx_i + b$

(unknown parameters)

The error (residual) =  $y_i - \hat{y}_i$

$$= y_i - (mx_i + b)$$

$$= y_i - mx_i - b$$

sum of all squared errors:

$$S(m, b) = \sum_{i=1}^n (y_i - mx_i - b)^2$$

we want to minimize this error  $\rightarrow$

Goal: find  $m$  &  $b$  for which  $S(m, b)$  minimum

so, we need partial derivatives,

$$\frac{\partial S}{\partial b} = \sum_{i=1}^n -2 (y_i - mx_i - b)$$

for minimum,  $\frac{\partial S}{\partial b} = 0$

$$\Rightarrow \sum_{i=1}^n y_i - mx_i - b = 0 \quad \text{--- (1)}$$



similarly:

$$\frac{\partial S}{\partial m} = \sum_{i=1}^n 2(y_i - mx_i - b)(-x_i) = 0$$

$$\Rightarrow \sum_{i=1}^n x_i (y_i - mx_i - b) = 0 \quad \text{--- (ii)}$$

solve the system:

① (i)  $\sum_{i=1}^n y_i - mx_i - b = 0$

$$\Rightarrow \sum_{i=1}^n y_i - m \sum_{i=1}^n x_i - nb = 0$$

$$\Rightarrow b = \frac{1}{n} \left( \sum_{i=1}^n y_i - m \sum_{i=1}^n x_i \right)$$

$$\Rightarrow \boxed{b = \bar{y} - m\bar{x}}$$

↘ ↗ average as  $\bar{y} = \frac{\sum y}{n}$

(ii)  $\sum_{i=1}^n x_i (y_i - mx_i - b) = 0$

$$\Rightarrow \sum_{i=1}^n x_i (y_i - mx_i - \bar{y} + m\bar{x}) = 0$$

$$\Rightarrow \sum_{i=1}^n x_i [(y_i - \bar{y}) - m(x_i - \bar{x})] = 0$$

$$\Rightarrow \sum x_i (y_i - \bar{y}) - m \sum x_i (x_i - \bar{x}) = 0$$



Proof of  $\sum x_i - n\bar{x} = 0$

$$\bar{x} = \frac{1}{n} \sum x_i$$

$$\Rightarrow \sum x_i = n\bar{x}$$

$$\therefore \sum (x_i - \bar{x}) = \sum_{i=1}^n x_i - \sum_{i=1}^n \bar{x}$$

$$\Rightarrow n\bar{x} - n\bar{x}$$

$$= 0$$

we have:

$$\sum x_i(x_i - \bar{x}) = \sum (x_i - \bar{x} + \bar{x})(x_i - \bar{x})$$

$$= \sum (x_i - \bar{x})^2 + \sum \bar{x}(x_i - \bar{x})$$

$$= \sum (x_i - \bar{x})^2 + \bar{x} \sum (x_i - \bar{x}) \rightarrow 0$$

$$= \sum (x_i - \bar{x})^2$$

similarly,

$$\sum x_i(y_i - \bar{y}) = \sum (x_i - \bar{x} + \bar{x})(y_i - \bar{y})$$

$$= \sum (x_i - \bar{x})(y_i - \bar{y}) + \bar{x} \sum (y_i - \bar{y}) \rightarrow 0$$



$$= \sum (x_i - \bar{x})(y_i - \bar{y})$$

$\therefore$  the eqn become  $\rightarrow$

$$\sum (x_i - \bar{x})(y_i - \bar{y}) - m \sum (x_i - \bar{x})^2 = 0$$

$$\Rightarrow m = \frac{\sum (x_i - \bar{x})(y_i - \bar{y})}{\sum (x_i - \bar{x})^2}$$

$$b = \bar{y} - m\bar{x}$$